Start moving code to the right places

TestModels/Streaming/src/SimpleStreamingImpl.dfy
@@ -1,59 +1,44 @@
 
 
+include "../Model/SimpleStreamingTypes.dfy"
 
-module StdLib {
-
-  // TODO: Add to actual Actions library:
-  // useful pattern to add an Action<Command, Result> facade
-  // to a set of methods that participate in a protocol.
-  // Then you have a history that ties the behavior
-  // of the methods together,
-  // supporting constraints on the order of calls etc.
-  trait Action<T, R> {
-    ghost var history: seq<(T, R)>
-
-    predicate Consumes(history: seq<(T, R)>, next: T)
-    predicate Produces(history: seq<(T, R)>)
-    
-
-    method Call(t: T) returns (r: R)
-      // requires Consumes(history, t)
-
-  }
-
-  // TODO: could use different words for calling when there is no input/no output
-  method Call<T>(a: Action<T, ()>, t: T) {
-    var _ := a.Call(t);
-  }
-
-  type SingleUseAction<T, R> = a: Action<T, R>
-    // TODO: Needs indirection or (!new)
-    // TODO: Not quite right, SingleUseAction should be a way of saying
-    // "I will only call this once"
-    // | forall history | a.Produces(history) :: |history| <= 1
-    | true 
-    witness *
-
-  predicate ConsumesAnything<T(!new), R(!new)>(a: Action<T, R>) {
-    forall history, next | a.Produces(history) :: a.Consumes(history, next)
-  }
-
-  // TODO: consumes any None-terminated sequence of inputs
-  predicate ConsumesTerminated<T(!new), R(!new)>(a: Action<Option<T>, R>)
-
-  type byte = b: nat | b < 256
-  type bytes = seq<byte>
-
-  datatype Option<T> = Some(value: T) | None
-  datatype Result<T, E> = Success(value: T) | Failure(error: E)
+module SimpleStreamingImpl refines AbstractSimpleStreamingOperations  {
+    datatype Config = Config
+    type InternalConfig = Config
+    predicate ValidInternalConfig?(config: InternalConfig)
+    {true}
+    function ModifiesInternalConfig(config: InternalConfig) : set<object>
+    {{}}
+    predicate GetStringEnsuresPublicly(input: GetStringInput, output: Result<GetStringOutput, Error>) {
+        true
+    }
+    predicate GetStringKnownValueEnsuresPublicly(input: GetStringInput, output: Result<GetStringOutput, Error>) {
+        true
+    }
+    predicate GetStringUTF8EnsuresPublicly(input: GetStringInput, output: Result<GetStringOutput, Error>) {
+        true
+    }
+    method GetString ( config: InternalConfig,  input: GetStringInput )
+    returns (output: Result<GetStringOutput, Error>) {
+        var res := GetStringOutput(value := input.value);
+        return Success(res);
+    }
+    method GetStringKnownValue ( config: InternalConfig,  input: GetStringInput )
+    returns (output: Result<GetStringOutput, Error>) {
+        expect input.value.Some?;
+        expect input.value.value == "TEST_SIMPLE_STRING_KNOWN_VALUE"; // This is done so as to assert that polymorph layer is doing one way conversion right as well.
+        var res := GetStringOutput(value := input.value);
+        return Success(res);
+    }
+    method GetStringUTF8 ( config: InternalConfig,  input: GetStringInput )
+    returns (output: Result<GetStringOutput, Error>) {
+        expect input.value.Some?;
+        var res := GetStringOutput(value := input.value);
+        return Success(res);
+    }
 }
 
 module Foo {
-
-  import opened StdLib  
-
-  datatype StreamingBlobRequest = StreamingBlobRequest()
-  datatype StreamingBlobResponse = StreamingBlobResponse()
 
   type Error
 
