TestModels/dafny-dependencies/StandardLibrary/src/Actions.dfy
@@ -1,0 +1,45 @@
+
+include "../../libraries/src/Wrappers.dfy"
+
+module StandardLibrary.Actions {
+
+  import opened Wrappers
+
+  // TODO: Add to actual Actions library:
+  // useful pattern to add an Action<Command, Result> facade
+  // to a set of methods that participate in a protocol.
+  // Then you have a history that ties the behavior
+  // of the methods together,
+  // supporting constraints on the order of calls etc.
+  trait Action<T, R> {
+    ghost var history: seq<(T, R)>
+
+    predicate Consumes(history: seq<(T, R)>, next: T)
+    predicate Produces(history: seq<(T, R)>)
+    
+
+    method Call(t: T) returns (r: R)
+      // requires Consumes(history, t)
+
+  }
+
+  // TODO: could use different words for calling when there is no input/no output
+  method Call<T>(a: Action<T, ()>, t: T) {
+    var _ := a.Call(t);
+  }
+
+  type SingleUseAction<T, R> = a: Action<T, R>
+    // TODO: Needs indirection or (!new)
+    // TODO: Not quite right, SingleUseAction should be a way of saying
+    // "I will only call this once"
+    // | forall history | a.Produces(history) :: |history| <= 1
+    | true 
+    witness *
+
+  predicate ConsumesAnything<T(!new), R(!new)>(a: Action<T, R>) {
+    forall history, next | a.Produces(history) :: a.Consumes(history, next)
+  }
+
+  // TODO: consumes any None-terminated sequence of inputs
+  predicate ConsumesTerminated<T(!new), R(!new)>(a: Action<Option<T>, R>)
+}
